Prove abstraction-based specs for TD.Read

Shallow/ReplicatedDisk.v
@@ -4,6 +4,7 @@ Require Import Disk.
 Require Import Automation.
 
 Require Import Shallow.ProgLang.Prog.
+Require Import Shallow.ProgLang.Hoare.
 Require Import Shallow.TwoDiskProg.
 Require Import Shallow.SeqDiskProg.
 
@@ -88,6 +89,115 @@ Module RD.
     intros; subst.
     unfold abstraction.
     destruct matches; simpl in *; try congruence.
+  Qed.
+
+  Definition first_disk_failed state :=
+    TD.disk0 state = None.
+
+  Lemma abstraction_d1_eq : forall state d a v,
+      first_disk_failed state ->
+      TD.disk1 state = Some d ->
+      d a = v ->
+      D.sdisk (abstraction state) a = v.
+  Proof.
+    unfold first_disk_failed; intros; subst.
+    unfold abstraction.
+    destruct matches; simpl in *; try congruence.
+  Qed.
+
+  Hint Resolve abstraction_preserved_bg_step.
+
+  Theorem TDRead0_ok : forall a,
+      prog_spec TD.step
+                (fun (_:unit) (state:TD.State) =>
+                   {|
+                     pre := invariant state;
+                     post := fun r state' =>
+                               abstraction state' = abstraction state /\
+                               invariant state' /\
+                               match r with
+                               | Working v => forall v0, D.sdisk (abstraction state) a = Some v0 ->
+                                                   v = v0
+                               | Failed => first_disk_failed state'
+                               end;
+                     crash := fun state' => abstraction state' = abstraction state;
+                   |})
+                (Prim (TD.Read d0 a)).
+  Proof.
+    intros.
+    unfold prog_spec; simpl; intros.
+    inv_exec; eauto.
+    TD.inv_step; cbn [TD.get_disk] in *.
+    intuition eauto.
+
+    destruct matches in *|-; intros; eauto.
+    eapply abstraction_d0_eq in Heqo; eauto.
+    erewrite abstraction_preserved_bg_step in * by eauto.
+    congruence.
+
+    repeat deex; intros; eauto.
+    eapply abstraction_d0_eq in Heqo; eauto.
+    erewrite abstraction_preserved_bg_step in * by eauto.
+    congruence.
+
+    TD.inv_step.
+    intuition eauto.
+  Qed.
+
+  Lemma bg_step_after_fail : forall state state',
+      first_disk_failed state ->
+      TD.bg_step state state' ->
+      state' = state.
+  Proof.
+    unfold first_disk_failed.
+    inversion 2; subst; simpl in *;
+      congruence.
+  Qed.
+
+  Lemma first_disk_failed_other_not_none : forall state,
+      first_disk_failed state ->
+      ~TD.disk1 state = None.
+  Proof.
+    unfold first_disk_failed; destruct state; simpl; intros.
+    deex; intuition congruence.
+  Qed.
+
+  Theorem TDRead1_ok : forall a,
+      prog_spec TD.step
+                (fun (_:unit) (state:TD.State) =>
+                   {|
+                     pre := invariant state /\
+                            first_disk_failed state;
+                     post := fun r state' =>
+                               abstraction state' = abstraction state /\
+                               invariant state' /\
+                               match r with
+                               | Working v => forall v0, D.sdisk (abstraction state) a = Some v0 ->
+                                                   v = v0
+                               | Failed => False
+                               end;
+                     crash := fun state' => abstraction state' = abstraction state;
+                   |})
+                (Prim (TD.Read d1 a)).
+  Proof.
+    unfold prog_spec; cbn [pre post crash]; intuition.
+    inv_exec; eauto.
+    TD.inv_step; cbn [TD.get_disk] in *.
+    intuition eauto.
+    eapply bg_step_after_fail in H; eauto; subst.
+
+    destruct matches in *|-; intros; eauto.
+    eapply abstraction_d1_eq in Heqo; eauto.
+    congruence.
+
+    repeat deex; intros; eauto.
+    eapply abstraction_d1_eq in Heqo; eauto.
+    congruence.
+
+    eapply first_disk_failed_other_not_none; eauto.
+
+    TD.inv_step.
+    intuition eauto.
   Qed.
 
   Theorem RD_ok : interpretation
